Refactor: add fractional points-tos to GC (no update laws yet); make all examples work

theories/interop/gctoken.v
@@ -1,6 +1,6 @@
 From Coq Require Import ssreflect.
 From stdpp Require Import strings gmap.
-From melocoton Require Import named_props.
+From melocoton Require Import named_props stdpp_extra.
 From transfinite.base_logic.lib Require Import ghost_map ghost_var.
 From iris.algebra Require Import gset.
 From iris.proofmode Require Import proofmode.
@@ -66,23 +66,24 @@ Definition SI_block_level_old (ζ_future : lstore) (χ_future : lloc_map) : iPro
   ∗ "%Hother_blocks" ∷ ⌜dom ζvirt ⊆ dom χ_future⌝
   ∗ "%Hstore" ∷ ⌜is_store χ_future ζ_future σMLvirt⌝.
 
-Definition per_location_invariant (ζ_future : lstore) (σMLvirt : store)
+Definition per_location_invariant (ζ_future : lstore) (σMLvirt : store) (dirty : gset lloc)
      (γ : lloc) (ℓ : loc) : iProp Σ :=
   ∃ (vs : list val) tg lvs, 
     ( ℓ ↦M/ ∗ ⌜ζ_future !! γ = Some (Bvblock (Mut, (tg, lvs)))⌝)
   ∨ (⌜σMLvirt !! ℓ = Some (Some vs)⌝ ∗ (γ ↦mut (tg, lvs)) ∗ lvs ~~∗ vs ∗ ⌜tg = TagDefault⌝)
+  ∨ (∃ (q r : Qp), ℓ ↦∗{# q} vs ∗ (γ ↦mut{DfracOwn r} (tg, lvs)) ∗ lvs ~~∗ vs ∗ ⌜tg = TagDefault⌝ ∗ ⌜(q+r=1)%Qp⌝ ∗ ⌜γ ∈ dirty⌝)
   ∨ (⌜σMLvirt !! ℓ = None⌝ ∗ ⌜ζ_future !! γ = None⌝)
   ∨ (⌜σMLvirt !! ℓ = Some None⌝ ∗ ⌜ζ_future !! γ = None⌝).
 (* the last two are "phony cases" -- they should not exist, but we do not control χ good enough in the op sem *)
 
-Definition SI_block_level (ζ_future : lstore) (χ_future : lloc_map) : iProp Σ :=
+Definition SI_block_level (ζ_future : lstore) (χ_future : lloc_map) (dirty : gset lloc) : iProp Σ :=
   ∃ (σMLvirt : store),
     "GCχauth" ∷ lloc_own_auth χ_future
   ∗ "GCζauth" ∷ lstore_own_auth ζ_future
   ∗ "%Hother_blocks" ∷ ⌜dom ζ_future ⊆ dom χ_future⌝
   ∗ "GCσMLv" ∷ state_interp (σMLvirt : language.language.state ML_lang)
   ∗ "GC_per_loc" ∷ ([∗ map] γ↦ℓ ∈ lloc_map_pubs χ_future,
-      per_location_invariant ζ_future σMLvirt γ ℓ)
+      per_location_invariant ζ_future σMLvirt dirty γ ℓ)
   ∗ "%Hstore" ∷ ⌜∀ ℓ, ℓ ∈ dom σMLvirt → ∃ γ, χ_future !! γ = Some (LlocPublic ℓ)⌝.
 
 Definition SI_GC (ζ_future : lstore) (θ : addr_map) (roots_s : gset addr) : iProp Σ :=
@@ -93,7 +94,7 @@ Definition SI_GC (ζ_future : lstore) (θ : addr_map) (roots_s : gset addr) : iP
   ∗ "%Hrootslive" ∷ ⌜roots_are_live θ roots_m⌝
   ∗ "%HGCOK" ∷ ⌜GC_correct ζ_future θ⌝.
 
-Definition GC (θ : addr_map) : iProp Σ :=
+Definition GC (θ : addr_map) (dirty : gset lloc) : iProp Σ :=
   ∃ (ζ ζ_future : lstore) (χ χ_future : lloc_map)
     (roots_s : gset addr),
     "GCζ" ∷ ghost_var wrapperG_γζ (1/2) ζ
@@ -101,11 +102,154 @@ Definition GC (θ : addr_map) : iProp Σ :=
   ∗ "GCθ" ∷ ghost_var wrapperG_γθ (1/2) θ
   ∗ "GCroots" ∷ ghost_var wrapperG_γroots_set (1/2) roots_s
   ∗ "GCinit" ∷ ghost_var wrapperG_γat_init (1/2) false
-  ∗ "HSI_block_level" ∷ SI_block_level ζ_future χ_future
+  ∗ "HSI_block_level" ∷ SI_block_level ζ_future χ_future dirty
   ∗ "HSI_GC" ∷ SI_GC ζ_future θ roots_s
   ∗ "%Hζfuture" ∷ ⌜freeze_lstore ζ ζ_future⌝
   ∗ "%Hχfuture" ∷ ⌜expose_llocs χ χ_future⌝.
 
 Definition at_init := ghost_var wrapperG_γat_init (1/2) true.
+
+Section Laws.
+
+Lemma GC_per_loc_modify_σ M ζ σMLvirt dirty γ ℓ' v:
+  gmap_inj M →
+  M !! γ = Some ℓ' →
+(([∗ map] ℓ↦y ∈ delete γ M, per_location_invariant ζ σMLvirt dirty ℓ y)
+⊢ [∗ map] ℓ↦y ∈ delete γ M, per_location_invariant ζ (<[ ℓ' := v ]> σMLvirt) dirty ℓ y)%I.
+Proof.
+  iIntros (Hinj Hlu) "Hbig".
+  iApply (big_sepM_wand with "Hbig").
+  iApply (big_sepM_intro).
+  iIntros "!>" (γ2 ℓ (Hne&Hlu2)%lookup_delete_Some) "(%vs'&%tg&%lvs&[(Hℓ&#Hsim)|[(%Hℓσ&Hγ&#Hsim)|[HH|[(%Hnone1&%Hnone2)|(%Hnone1&%Hnone2)]]]])"; iExists vs', tg, lvs.
+  - iLeft; by iFrame.
+  - iRight. iLeft. iFrame "Hγ Hsim". iPureIntro.
+    rewrite lookup_insert_ne; first done.
+    intros ->. by eapply Hne, Hinj.
+  - iRight. iRight. iLeft. done.
+  - iRight. iRight. iRight. iLeft. iPureIntro. split; last done.
+    rewrite lookup_insert_ne; try done.
+    intros ->. by eapply Hne, Hinj.
+  - iRight. iRight. iRight. iRight. iFrame. iPureIntro; split; last done.
+    rewrite lookup_insert_ne; first done.
+    intros ->. by eapply Hne, Hinj.
+Qed.
+
+Lemma GC_per_loc_insert M ζ σMLvirt dirty ℓ' v:
+  (∀ γ, M !! γ ≠ Some ℓ') →
+(([∗ map] γ↦ℓ ∈ M, per_location_invariant ζ σMLvirt dirty γ ℓ)
+⊢ [∗ map] γ↦ℓ ∈ M, per_location_invariant ζ (<[ ℓ' := v ]> σMLvirt) dirty γ ℓ)%I.
+Proof.
+  iIntros (Hnℓ) "Hbig".
+  iApply (big_sepM_wand with "Hbig").
+  iApply (big_sepM_intro).
+  iIntros "!>" (γ2 ℓ Hne) "(%vs'&%tg&%lvs&[(Hℓ&#Hsim)|[(%Hℓσ&Hγ&#Hsim)|[HH|[(%Hnone1&%Hnone2)|(%Hnone1&%Hnone2)]]]])"; iExists vs', tg, lvs.
+  - iLeft; by iFrame.
+  - iRight. iLeft. iFrame "Hγ Hsim". iPureIntro.
+    rewrite lookup_insert_ne; first done.
+    intros ->. eapply Hnℓ, Hne.
+  - iRight. iRight. iLeft. done.
+  - iRight. iRight. iRight. iLeft. iSplit; last done. iPureIntro.
+    rewrite lookup_insert_ne; try done.
+    intros ->. eapply Hnℓ, Hne.
+  - do 4 iRight. iFrame. iPureIntro; split; last done.
+    rewrite lookup_insert_ne; first done.
+    intros ->. by eapply Hnℓ, Hne.
+Qed.
+
+Lemma GC_per_loc_modify_ζ M ζ σMLvirt dirty γ v:
+  M !! γ = None →
+(([∗ map] ℓ↦y ∈ M, per_location_invariant ζ σMLvirt dirty ℓ y)
+⊢ [∗ map] ℓ↦y ∈ M, per_location_invariant (<[ γ := v ]> ζ) σMLvirt dirty ℓ y)%I.
+Proof.
+  iIntros (Hne) "Hbig".
+  iApply (big_sepM_wand with "Hbig").
+  iApply (big_sepM_intro).
+  iIntros "!>" (γ2 ℓ Hle) "(%vs'&%tg&%lvs&[(Hℓ&#Hsim)|[(%Hℓσ&Hγ&Hsim&%Heq)|[HH|[(%Hnone1&%Hnone2)|(Hnone1&%Hnone2)]]]])"; iExists vs', tg, lvs.
+  - iLeft. iFrame. rewrite lookup_insert_ne; first done.
+    intros ->; congruence.
+  - iRight. iLeft. by iFrame.
+  - iRight. iRight. iLeft. done.
+  - iRight. iRight. iRight. iLeft. iPureIntro; split; first done.
+    rewrite lookup_insert_ne; try done.
+    intros ->. simplify_eq.
+  - do 4 iRight. iFrame. iPureIntro.
+    rewrite lookup_insert_ne; try done.
+    intros ->. simplify_eq.
+Qed.
+
+Lemma GC_per_loc_modify_ζ_in_detail M ζ σMLvirt dirty γ tg' lvs':
+ζ !! γ ≠ None →
+(([∗ map] ℓ↦y ∈ M, per_location_invariant ζ σMLvirt dirty ℓ y)
+⊢ [∗ map] ℓ↦y ∈ M, per_location_invariant (<[ γ := (Bvblock (Mut, (tg', lvs'))) ]> ζ) σMLvirt dirty ℓ y)%I.
+Proof.
+  iIntros (Hne) "Hbig".
+  iApply (big_sepM_wand with "Hbig").
+  iApply (big_sepM_intro).
+  iIntros "!>" (γ2 ℓ Hle) "(%vs'&%tg&%lvs&[(Hℓ&%Hsim)|[(%Hℓσ&Hγ&Hsim&%Heq)|[HH|[(%Hnone1&%Hnone2)|(%Hnone1&%Hnone2)]]]])";
+  (destruct (decide (γ2 = γ)) as [Hl|Hr]; [subst γ2|]; iExists vs'); try (by simplify_eq).
+  - iExists tg', lvs'. iLeft. iFrame. iPureIntro. rewrite lookup_insert. done.
+  - iExists tg, lvs. iLeft. iFrame. iPureIntro. rewrite lookup_insert_ne; try done.
+  - iExists tg, lvs. iRight. iLeft. iFrame. by iPureIntro.
+  - iExists tg, lvs. iRight. iLeft. iFrame. by iPureIntro.
+  - iExists tg, lvs. iRight. iRight. iLeft. iFrame.
+  - iExists tg, lvs. iRight. iRight. iLeft. iFrame.
+  - iExists tg', lvs'. iRight. iRight. iRight. iLeft. rewrite lookup_insert_ne; done.
+  - iExists tg', lvs'. iRight. iRight. iRight. iRight. rewrite lookup_insert_ne; done.
+Qed.
+
+Lemma GC_per_loc_make_dirty M ζ σMLvirt dirty dirty':
+  dirty ⊆ dirty' →
+(([∗ map] γ↦ℓ ∈ M, per_location_invariant ζ σMLvirt dirty γ ℓ)
+⊢ [∗ map] γ↦ℓ ∈ M, per_location_invariant ζ σMLvirt dirty' γ ℓ)%I.
+Proof.
+  iIntros (Hnℓ) "Hbig".
+  iApply (big_sepM_wand with "Hbig").
+  iApply (big_sepM_intro).
+  iIntros "!>" (γ2 ℓ Hne) "(%vs'&%tg&%lvs&[(Hℓ&#Hsim)|[(%Hℓσ&Hγ&#Hsim&%Heq)|[(%q&%r&Hmapsℓ&Hmapsγ&#Hsim&%Heq&%Hsum&%Hdirty)|[(%Hnone1&%Hnone2)|(%Hnone1&%Hnone2)]]]])"; iExists vs', tg, lvs.
+  - iLeft; by iFrame.
+  - iRight. iLeft. iFrame "Hγ Hsim". iPureIntro. done.
+  - iRight. iRight. iLeft. iExists q,r. iFrame. iFrame "Hsim". iPureIntro; split_and!; try done.
+    by eapply elem_of_weaken.
+  - iRight. iRight. iRight. iLeft. iSplit; last done. iPureIntro. done.
+  - do 4 iRight. iFrame. iPureIntro; done.
+Qed.
+
+Lemma GC_per_loc_remove_dirty M ζ σMLvirt dirty γ':
+  M !! γ' = None →
+(([∗ map] γ↦ℓ ∈ M, per_location_invariant ζ σMLvirt dirty γ ℓ)
+⊢ [∗ map] γ↦ℓ ∈ M, per_location_invariant ζ σMLvirt (dirty ∖ {[ γ' ]}) γ ℓ)%I.
+Proof.
+  iIntros (Hnℓ) "Hbig".
+  iApply (big_sepM_wand with "Hbig").
+  iApply (big_sepM_intro).
+  iIntros "!>" (γ2 ℓ Hne) "(%vs'&%tg&%lvs&[(Hℓ&#Hsim)|[(%Hℓσ&Hγ&#Hsim&%Heq)|[(%q&%r&Hmapsℓ&Hmapsγ&#Hsim&%Heq&%Hsum&%Hdirty)|[(%Hnone1&%Hnone2)|(%Hnone1&%Hnone2)]]]])"; iExists vs', tg, lvs.
+  - iLeft; by iFrame.
+  - iRight. iLeft. iFrame "Hγ Hsim". iPureIntro. done.
+  - iRight. iRight. iLeft. iExists q,r. iFrame. iFrame "Hsim". iPureIntro; split_and!; try done.
+    eapply elem_of_difference; split; first done. eapply not_elem_of_singleton; intros HH; simplify_eq.
+  - iRight. iRight. iRight. iLeft. iSplit; last done. iPureIntro. done.
+  - do 4 iRight. iFrame. iPureIntro; done.
+Qed.
+
+Lemma GC_per_loc_delete_ζ M ζ σMLvirt dirty γ:
+  M !! γ = None →
+(([∗ map] ℓ↦y ∈ M, per_location_invariant ζ σMLvirt dirty ℓ y)
+⊢ [∗ map] ℓ↦y ∈ M, per_location_invariant (delete γ ζ) σMLvirt dirty ℓ y)%I.
+Proof.
+  iIntros (Hne) "Hbig".
+  iApply (big_sepM_wand with "Hbig").
+  iApply (big_sepM_intro).
+  iIntros "!>" (γ2 ℓ Hle) "(%vs'&%tg&%lvs&[(Hℓ&#Hsim)|[(%Hℓσ&Hγ&Hsim&%Heq)|[HH|[(%Hnone1&%Hnone2)|(Hnone1&%Hnone2)]]]])"; iExists vs', tg, lvs.
+  - iLeft. iFrame. rewrite lookup_delete_ne; first done.
+    intros ->; congruence.
+  - iRight. iLeft. by iFrame.
+  - iRight. iRight. iLeft. iFrame.
+  - iRight. iRight. iRight. iLeft. iPureIntro; split; first done.
+    rewrite lookup_delete_ne; try done.
+    intros ->. simplify_eq.
+  - do 4 iRight. iFrame. iPureIntro. apply lookup_delete_None; by right.
+Qed.
+
+End Laws.
 
 End GCtoken.
