theories/interop/wp_prims/alloc_foreign.v
@@ -29,7 +29,7 @@ Proof using.
   iIntros (Φ') "Hb Hcont". iApply wp_wrap_call; first done. cbn [snd].
   rewrite weakestpre.wp_unfold. rewrite /weakestpre.wp_pre.
   iIntros "%σ Hσ". cbn -[wrap_prog].
-  SI_at_boundary. iNamed "HGC". SI_GC_agree.
+  SI_at_boundary. iNamed "HGC". SI_GC_agree. iNamed "HSI_GC". iNamed "HSI_block_level".
   iAssert (⌜∀ k lv, roots_m !! k = Some lv →
             ∃ w, mem !! k = Some (Storing w) ∧ repr_lval (θC ρc) lv w⌝)%I as "%Hroots".
   1: { iIntros (kk vv Hroots).
@@ -41,42 +41,36 @@ Proof using.
   { eapply GC_correct_transport_rev; last done; done. }
 
   iApply wp_pre_cases_c_prim; [done..|].
-  iExists (λ '(e', σ'), ∃ γ id χC' ζC' θC' (aret:loc) mem',
-      χC ρc !! γ = None ∧
-      (∀ γ' id', χC ρc !! γ' = Some (LlocForeign id') → id' ≠ id) ∧
-      χC' = <[ γ := LlocForeign id ]> (χC ρc) ∧
-      ζC' = <[ γ := Bforeign None ]> (ζC ρc) ∧
-      GC_correct ζC' θC' ∧
-      repr θC' roots_m privmem mem' ∧
-      roots_are_live θC' roots_m ∧
-      θC' !! γ = Some aret ∧
-      e' = WrSE (ExprV (# aret)) ∧
-      σ' = CState (WrapstateC χC' ζC' θC' (rootsC ρc)) mem').
+  iExists (λ '(e', σ'), ∃ γ fid χC' ζC' θC' (a:loc) mem',
+    χC ρc !! γ = None ∧
+    (∀ γ' id', χC ρc !! γ' = Some (LlocForeign id') → id' ≠ fid) ∧
+    χC' = <[γ := LlocForeign fid]> (χC ρc) ∧
+    ζC' = <[γ := Bforeign None]> (ζC ρc) ∧
+    GC_correct ζC' θC' ∧
+    repr θC' _ _ _ ∧
+    roots_are_live θC' _ ∧
+    θC' !! γ = Some a ∧
+    e' = WrSE (ExprV #a) ∧
+    σ' = CState {| χC := χC'; ζC := ζC'; θC := θC'; rootsC := rootsC ρc |} mem').
   iSplit. { iPureIntro. econstructor; naive_solver. }
-  iIntros (? ? ? (γ & id & χC' & ζC' & θC' & aret & mem' &
-                  HγNone & Hidfresh & -> & -> & HGCOK' & Hrepr' & Hrootslive' & ?)).
+  iIntros (? ? ? (γ & fid & χC' & ζC' & θC' & a & mem' &
+                  HγNone & Hfidfresh & -> & -> & HGCOK' & Hrepr' & Hrootslive' & ?)).
   destruct_and!; simplify_eq.
 
-  assert (χvirt !! γ = None) as Hχvirtγ.
-  { eapply not_elem_of_dom. destruct Hχvirt as [<- _].
+  assert (χ_future !! γ = None) as Hχfutγ.
+  { eapply not_elem_of_dom. destruct Hχfuture as [<- _].
     by eapply not_elem_of_dom. }
-  assert (ζσ !! γ = None) as Hζσγ.
-  { eapply not_elem_of_dom. destruct Hstore_blocks as [HHL HHR].
-    intros (ℓ&Vs&HX1&HX2)%HHR. congruence. }
-  assert (ζvirt !! γ = None) as Hζvirtγ.
-  { eapply not_elem_of_dom. intros H. eapply not_elem_of_dom in Hχvirtγ.
-    apply Hχvirtγ. eapply elem_of_weaken; first done. done. }
+  assert (ζ_future !! γ = None) as Hζfutγ.
+  { eapply not_elem_of_dom. eintros H%elem_of_weaken; last done.
+    by eapply not_elem_of_dom in Hχfutγ. }
   assert (ζC ρc !! γ = None) as HζCγ.
-  { destruct Hfreezeρ as [HL HR]. eapply not_elem_of_dom. rewrite HL.
-    rewrite dom_union_L.
-    intros [HH|HH]%elem_of_union.
-    all: eapply elem_of_dom in HH; destruct HH as [v HHv]; congruence. }
+  { destruct Hζfuture as [HL HR]. eapply not_elem_of_dom. rewrite HL.
+    eapply not_elem_of_dom in Hζfutγ; done. }
 
-  assert (freeze_lstore (<[γ := Bforeign None]> (ζC ρc)) (ζσ ∪ <[γ:=Bforeign None]> ζvirt)) as Hfreezeρ_new.
-  { destruct Hfreezeρ as [HfL HfR]; split.
-    - rewrite !dom_insert_L HfL dom_union_L. set_solver+.
-    - rewrite <- insert_union_r. 2: done.
-      intros γ1 b1 b2 ?%lookup_insert_Some ?%lookup_insert_Some.
+  eassert (freeze_lstore (<[γ := _]> (ζC ρc)) (<[γ:=_]> ζ_future)) as Hζfuturenew.
+  { destruct Hζfuture as [HfL HfR]; split.
+    - by erewrite !dom_insert_L, HfL.
+    - intros γ1 b1 b2 ?%lookup_insert_Some ?%lookup_insert_Some.
       destruct_or!; destruct_and!; simplify_eq; eauto. }
 
   iMod (set_to_none _ _ _ _ Hpriv with "HσC GCrootspto") as "(HσC&GCrootspto)".
@@ -86,48 +80,38 @@ Proof using.
   iMod (ghost_var_update_halves with "GCχ SIχ") as "(GCχ&SIχ)".
   iMod (ghost_var_update_halves with "GCθ SIθ") as "(GCθ&SIθ)".
 
-  iMod (lstore_own_insert _ γ (Bforeign None) with "GCζvirt") as "(GCζvirt & Hbp1)". 1: done.
-  iMod (lloc_own_allocate_foreign _ γ id with "[] GCχvirt") as "(GCχvirt&Hbp2)". 1: done.
+  iMod (lstore_own_insert _ γ _ with "GCζauth") as "(GCζauth & Hbp1)". 1: done.
+  iMod (lloc_own_allocate_foreign _ γ fid with "[] GCχauth") as "(GCχauth&Hbp2)". 1: done.
 
   do 3 iModIntro. iFrame. cbn -[wrap_prog].
   iSplitL "SIinit". { iExists false. iFrame. }
   iApply wp_value; first done.
   iApply "Hcont". iFrame.
-  iApply ("Cont" $! θC' γ with "[-Hbp2 Hbp1] [Hbp2 Hbp1] []"); try done.
+  iApply ("Cont" $! θC' γ with "[-Hbp2 Hbp1] [Hbp2 $Hbp1] []"); try done.
   3: iPureIntro; by econstructor.
-  2: iFrame; by eauto.
+  2: iSplit; try done; by iExists _.
   rewrite /GC /named.
-  iExists _, _, (ζσ), (<[γ:=Bforeign None]> ζvirt), _, (<[γ:=LlocForeign id]> χvirt).
-  iExists σMLvirt, _, _.
-  rewrite pub_locs_in_lstore_alloc_foreign //. iFrame.
-  iPureIntro; split_and!; eauto.
-  2: destruct Hstore_blocks as [HsL HsR]; split.
-  - eapply map_disjoint_insert_r. split; done.
-  - intros ℓ Hdom. destruct (HsL ℓ Hdom) as (γ1 & Hγ1). exists γ1. rewrite lookup_insert_ne; first done.
-    intros ->; congruence.
-  - intros γ1; split.
-    + intros (ℓ&Vs&HH1&HH2)%HsR. exists ℓ,Vs; split; try done.
-      rewrite lookup_insert_ne; first done. intros ->; congruence.
-    + intros (ℓ&Vs&[[??]|[??]]%lookup_insert_Some&HH2); try congruence.
-      eapply HsR. by exists ℓ,Vs.
-  - erewrite !dom_insert_L. clear -Hother_blocks. set_solver.
-  - intros ℓ vs γ1 blk1 HH1 [[??]|[? HH2]]%lookup_insert_Some HH3; try congruence.
-    rewrite -!insert_union_r in HH3|-*; try done.
-    rewrite lookup_insert_ne in HH3; last done.
-    specialize (Hstore ℓ vs γ1 blk1 HH1 HH2 HH3).
-    inversion Hstore; subst. econstructor.
-    eapply Forall2_impl; first eassumption.
-    intros vml vl HH4. eapply is_val_mono. 3: apply HH4.
-    + eapply insert_subseteq. done.
-    + eapply insert_subseteq. eapply lookup_union_None; done.
-  - apply expose_llocs_insert_both; eauto. intros γ' ? _ HH1 ->.
-    destruct Hχvirt as (Hdom & ? & Hexp).
-    assert (is_Some (χC ρc !! γ')) as [? HH2].
-    { rewrite -elem_of_dom Hdom elem_of_dom //. }
-    specialize (Hexp _ _ _ HH2 HH1). inversion Hexp; simplify_eq.
-    naive_solver.
-  - cbn. by apply lloc_map_inj_insert_foreign.
-  - eapply GC_correct_transport; done.
+  do 5 iExists _. iFrame.
+  iSplitL "GCσMLv GC_per_loc". 2: iSplit; last iSplit; try iPureIntro.
+  - iExists σMLvirt. iFrame.
+    iPoseProof (GC_per_loc_modify_ζ with "GC_per_loc") as "GC_per_loc".
+    1: apply lloc_map_pubs_lookup_None; by left. unfold named.
+    repeat iSplit; try iPureIntro.
+    * rewrite dom_insert_L; set_solver.
+    * rewrite lloc_map_pubs_insert_foreign delete_notin.
+      2: apply lloc_map_pubs_lookup_None; by left. done.
+    * intros ℓ Hℓ; destruct (Hstore _ Hℓ) as (γ'&Hγ'); exists γ'; rewrite lookup_insert_ne; first done.
+      intros ->; simplify_eq.
+  - iExists roots_m. iFrame. iPureIntro; split_and!; try done.
+    by eapply GC_correct_transport.
+  - done.
+  - apply expose_llocs_insert_both; try done.
+    destruct Hχfuture as (Hf1&Hf2&Hf3).
+    intros γ' [|id'|] _ Hf Heq; simplify_eq.
+    edestruct (χC ρc !! γ') eqn:Heq.
+    2: eapply elem_of_dom_2 in Hf; eapply not_elem_of_dom in Heq; set_solver.
+    pose proof (Hf3 _ _ _ Heq Hf) as Hinv; inversion Hinv; simplify_eq.
+    by eapply (Hfidfresh γ' fid).
 Qed.
 
 End Laws.
