theories/interop/wp_prims/common.v
@@ -80,5 +80,19 @@ Proof.
   constructor; by eapply elem_of_list_lookup_2.
 Qed.
 
+Lemma HSI_GC_modify ζ θ roots γ blk':
+  (∀ γ', lval_in_block blk' (Lloc γ') → γ' ∈ dom θ ∨ ∃ blk, ζ !! γ = Some blk ∧ lval_in_block blk (Lloc γ')) →
+  SI_GC ζ θ roots
+⊢ SI_GC (<[ γ := blk' ]> ζ) θ roots.
+Proof.
+  iIntros (H) "H". iNamed "H".
+  iExists roots_m. iFrame. iPureIntro; split_and!; try done.
+  destruct HGCOK as [HL HR]; split; first done.
+  intros γ1 blk γ2 Hγ1 [(Heq&Hlu)|(Hne&Hlu)]%lookup_insert_Some H2; simplify_eq.
+  2: by eapply HR.
+  destruct (H _ H2) as [Hl|(blk1&Hblk&Hr)]; first done.
+  apply (HR _ _ _ Hγ1 Hblk Hr).
+Qed.
+
 
 End Laws.
